TODO.md
@@ -7,3 +7,6 @@
 [ ] syntax delab 
 [ ] make sure no user-land code is referenced in the framework lib (incrementBody, increment_body_lowers_ok)
 [ ] compilation proofs 
+[ ] handle proofs against oracle manipulation attacks 
+[ ] handle proofs against sandwitch attacks
+[ ] handle proofs against flashloans attacks
